manual example of repeated enum

example/enum.go
@@ -14,15 +14,29 @@ const (
 	STATUS_PROFESSOR   Status = 3
 )
 
+// Wrapper for type aliasing compliance
+func MarshalStatus(enc []byte, s Status) []byte {
+	return marshal.WriteInt(enc, uint64(s))
+}
+
+func UnmarshalStatus(s []byte) (Status, []byte) {
+	status_raw, s := marshal.ReadInt(s)
+	return Status(status_raw), s
+}
+
 type Person struct {
-	Name   string
-	Status Status
+	Name     string
+	Status   Status
+	Statuses []Status // Does this make sense? No, but I need to test repeated enums...
 }
 
 func MarshalPerson(enc []byte, p Person) []byte {
 	primitive.AssumeNoStringOverflow(p.Name)
 	enc = marshal.WriteLenPrefixedBytes(enc, []byte(p.Name))
 	enc = marshal.WriteInt(enc, uint64(p.Status))
+
+	enc = marshal.WriteInt(enc, uint64(len(p.Statuses)))
+	enc = marshal.WriteSlice[Status](enc, p.Statuses, MarshalStatus)
 	return enc
 }
 
@@ -30,9 +44,12 @@ func UnmarshalPerson(s []byte) (Person, []byte) {
 	name, s := marshal.ReadLenPrefixedBytes(s)
 	status_int, s := marshal.ReadInt(s)
 	status := Status(status_int)
+	statuses_len, s := marshal.ReadInt(s)
+	statuses, s := marshal.ReadSlice[Status](s, statuses_len, UnmarshalStatus)
 
 	return Person{
-		Name:   string(name),
-		Status: status,
+		Name:     string(name),
+		Status:   status,
+		Statuses: statuses,
 	}, s
 }
