example/proof/person_proof.v
@@ -34,19 +34,89 @@ Module Person_Proof.
       | STATUS_PROFESSOR => 3
       end.
 
+    Definition status_has_encoding (encoded:list u8) (args:Status) : Prop :=
+      encoded = u64_le $ to_tag $ args.
+
+    Definition status_own (args__v: example.Status.t) (args__c:Status) (dq:dfrac) : iProp Σ :=
+      "%Hstatus_eq" ∷ ⌜ args__v = to_tag args__c ⌝.
+
+    Lemma wp_Status_Encode (args__t: example.Status.t) (args__c:Status) (pre_sl: slice.t) (prefix: list u8) (dq: dfrac):
+      {{{
+            is_pkg_init example ∗
+            status_own args__t args__c dq ∗
+            own_slice pre_sl (DfracOwn 1) prefix ∗
+            own_slice_cap w8 pre_sl (DfracOwn 1)
+      }}}
+        @! example.MarshalStatus #pre_sl #args__t
+      {{{
+            enc enc_sl, RET #enc_sl;
+            ⌜ status_has_encoding enc args__c ⌝ ∗
+            status_own args__t args__c dq ∗
+            own_slice enc_sl (DfracOwn 1) (prefix ++ enc) ∗
+            own_slice_cap w8 enc_sl (DfracOwn 1)
+      }}}.
+
+    Proof.
+      wp_start as "(Hown & Hsl & Hcap)". unfold status_own. iNamed "Hown".
+      wp_auto.
+
+      wp_apply (wp_WriteInt with "[$Hsl $Hcap]").
+      iIntros (?) "[Hsl Hcap]". wp_auto.
+
+      iApply "HΦ". iFrame.
+      iPureIntro. unfold status_has_encoding.
+      rewrite Hstatus_eq.
+      split; try reflexivity.
+    Qed.
+
+    Lemma wp_Status_Decode (enc: list u8) (enc_sl: slice.t) (args__c:Status) (suffix: list u8) (dq: dfrac):
+      {{{
+            is_pkg_init example ∗
+            own_slice enc_sl dq (enc ++ suffix) ∗
+            ⌜ status_has_encoding enc args__c ⌝
+      }}}
+        @! example.UnmarshalStatus #enc_sl
+      {{{
+            args__t suff_sl, RET (#args__t, #suff_sl);
+            status_own args__t args__c (DfracOwn 1) ∗
+            own_slice suff_sl dq suffix
+      }}}.
+    Proof.
+      wp_start as "(Hsl & %Henc)". wp_auto.
+      unfold status_has_encoding in Henc.
+      rewrite Henc. 
+
+      wp_apply (wp_ReadInt with "[$Hsl]").
+      iIntros (?) "Hsl". wp_auto.
+
+      iApply "HΦ".
+      iFrame.
+      done.
+    Qed.
+
     Record C :=
       mkC {
         name' : go_string; 
         status' : Status;
+        statuses' : list Status;
       }.
 
     Definition has_encoding (encoded:list u8) (args:C) : Prop :=
-      encoded = (u64_le $ length args.(name')) ++ args.(name') ++ (u64_le (to_tag args.(status')))
-                                                               /\ length args.(name') < 2^64.
+      ∃ (statuses_enc : list u8),
+        encoded = (u64_le $ length args.(name')) ++ args.(name') ++ (u64_le (to_tag args.(status')))
+                                                           ++ (u64_le $ length $ args.(statuses'))
+                                                           ++ statuses_enc
+        /\ encodes statuses_enc args.(statuses') status_has_encoding
+        /\ length args.(name') < 2^64
+        /\ length args.(statuses') < 2^64.
       
     Definition own (args__v:example.Person.t) (args__c:C) (dq:dfrac) : iProp Σ :=
+      ∃ (l__statuses : list example.Status.t), 
       "%Hname" ∷ ⌜ args__v.(example.Person.Name') = args__c.(name') ⌝ ∗
-      "%Hstatus" ∷ ⌜ args__v.(example.Person.Status') = (to_tag args__c.(status')) ⌝.
+      "%Hstatus" ∷ ⌜ args__v.(example.Person.Status') = (to_tag args__c.(status')) ⌝ ∗
+      "Hown_statuses_sl" ∷ own_slice args__v.(example.Person.Statuses') dq l__statuses ∗
+      "Hown_statuses_own" ∷ ([∗ list] x;c ∈ l__statuses;args__c.(statuses'), status_own x c dq) ∗
+      "%Hown_statuses_len" ∷ ⌜ length l__statuses < 2^64 ⌝.
 
     Lemma wp_Enocde (args__t:example.Person.t) (args__c:C) (pre_sl:slice.t) (prefix:list u8) (dq:dfrac):
       {{{
@@ -78,11 +148,36 @@ Module Person_Proof.
       wp_apply (wp_WriteInt with "[$Hsl $Hcap]").
       iIntros (?) "[Hsl Hcap]". wp_auto.
 
-      iApply "HΦ". iFrame.
-      iSplit.
-      + done.
-      + rewrite -?app_assoc. rewrite Hname. rewrite Hstatus. iFrame.
-        done.
+      wp_apply (wp_WriteInt with "[$Hsl $Hcap]").
+      iIntros (?) "[Hsl Hcap]". wp_auto.
+
+      iDestruct (own_slice_len with "Hown_statuses_sl") as "%Hown_statuses_sz".
+      iDestruct (big_sepL2_length with "Hown_statuses_own") as "%Hown_statuses_sz'".
+      rewrite Hown_statuses_sz' in Hown_statuses_sz.
+      wp_apply (wp_WriteSlice with "[$Hsl $Hcap $Hown_statuses_sl $Hown_statuses_own]").
+      {
+        iIntros (????) "!>".
+        iIntros (?) "(Hown & Hsl & Hcap) HΦ".
+        wp_apply (wp_Status_Encode with "[$Hown $Hsl $Hcap]").
+        iApply "HΦ".
+      }
+      iIntros (statuses_enc statuses_sl') "(Hown_statuses & Hown_statuses_own & %Henc_statuses & Hsl & Hcap)".
+      wp_auto.
+
+      iApply "HΦ". rewrite -?app_assoc.
+      iFrame. iPureIntro.
+
+      unfold has_encoding.
+      split; last done.
+      exists statuses_enc.
+      split.
+      {
+        rewrite Hown_statuses_sz.
+        rewrite ?w64_to_nat_id.
+        congruence.
+      }
+      rewrite <- Hown_statuses_sz'.
+      done. 
     Qed.
 
     Lemma wp_Decode (enc: list u8) (enc_sl: slice.t) (args__c:C) (suffix: list u8) (dq: dfrac):
@@ -101,7 +196,7 @@ Module Person_Proof.
     Proof.
       wp_start as "(Hsl & %Henc)". wp_auto.
       unfold has_encoding in Henc.
-      destruct Henc as [Henc HnameLen].
+      destruct Henc as (statuses_enc & Henc & Hstatuses_enc & HnameLen & HstatusesLen).
       rewrite Henc. rewrite -?app_assoc.
 
       wp_apply (wp_ReadLenPrefixedBytes with "[$Hsl]"); first word.
@@ -110,6 +205,22 @@ Module Person_Proof.
       wp_apply (wp_ReadInt with "[$Hsl]").
       iIntros (?) "Hsl". wp_auto.
 
+      wp_apply (wp_ReadInt with "[$Hsl]").
+      iIntros (?) "Hsl". wp_auto.
+
+      wp_apply (wp_ReadSlice  with "[$Hsl]").
+      {
+        iSplit; auto.
+        iSplit; first word.
+        iIntros (????) "!>".
+        iIntros (?) "[Hsl Henc] HΦ".
+        wp_apply (wp_Status_Decode with "[$Hsl $Henc]").
+        iApply "HΦ".
+      }
+      iIntros (???) "(Hown_statuses_sl & Hown_statuses_own & Hsl)". wp_auto.
+      iDestruct (big_sepL2_length with "Hown_statuses_own") as "%Hown_statuses_sz".
+      rewrite <- Hown_statuses_sz in HstatusesLen.
+      
       wp_apply (wp_StringFromBytes with "[$Hn]").
       iIntros "Hn". wp_auto.
 
